src/lake/Lake/Build/Target/Fetch.lean
@@ -9,25 +9,76 @@ import Lake.Config.Monad
 
 namespace Lake
 
-protected def BuildKey.fetch (self : BuildKey) [h : FamilyOut BuildData self α] : FetchM (Job α) := do
-  match self_eq:self with
+private def BuildKey.fetchCore (self : BuildKey) : FetchM (Job (BuildData self)) := do
+  match self with
   | module modName =>
     let some mod ← findModule? modName
       | error s!"invalid target '{self}': module '{modName}' not found in workspace"
-    return cast (by rw [← h.fam_eq, self_eq]; simp) (Job.pure mod)
+    return Job.pure <| toFamily mod
   | package pkgName =>
     let some pkg ← findPackage? pkgName
       | error s!"invalid target '{self}': package '{pkgName}' not found in workspace"
-    return cast (by rw [← h.fam_eq, self_eq]; simp) (Job.pure pkg.toPackage)
-  | packageTarget pkgName targetName =>
+    return Job.pure <| toFamily pkg.toPackage
+  | packageTarget pkgName targetName dataKind =>
     let some pkg ← findPackage? pkgName
       | error s!"invalid target '{self}': package '{pkgName}' not found in workspace"
-    have : FamilyOut BuildData (pkg.target targetName).key α :=
-      ⟨by simpa [self_eq] using h.fam_eq⟩
-    fetch <| pkg.target targetName
-  | facet key targetKind facetName =>
-    -- TODO: Support this
-    error s!"unsupported target '{self}': fetching builtin targets by key is not currently supported"
+    match dataKind with
+    | .anonymous =>
+      fetch <| pkg.target targetName
+    | `leanLib =>
+      let some lib := pkg.findLeanLib? targetName
+        | error s!"invalid target '{self}': Lean library '{targetName}' not found in package '{pkgName}'"
+      return Job.pure <| toFamily lib
+    | `leanExe =>
+      let some exe := pkg.findLeanExe? targetName
+        | error s!"invalid target '{self}': Lean executable '{targetName}' not found in package '{pkgName}'"
+      return Job.pure <| toFamily exe
+    | `externLib =>
+      let some lib := pkg.findExternLib? targetName
+        | error s!"invalid target '{self}': External library '{targetName}' not found in package '{pkgName}'"
+      return Job.pure <| toFamily lib
+    | _ =>
+      error s!"invalid target '{self}': unknown data kind '{dataKind}'"
+  | facet target facetName dataKind =>
+    let .anonymous := dataKind
+      | error s!"invalid target '{self}': facets do not currently support non-anonymous data kinds"
+    if h : target.kind.isAnonymous then
+      error s!"invalid target '{self}': facet of opaque target kind '{target.kind}'"
+    else
+      let job ← target.fetchCore
+      let job : Job (TargetData target.kind) :=
+        cast (by rw [target.data_eq_of_kind h]) job
+      match kind_eq:target.kind with
+      | `leanLib =>
+        let job : Job LeanLib := cast (by simp [kind_eq]) job
+        let job ← job.bindM fun lib => fetch (.libraryFacet lib facetName)
+        return cast (by simp [kind_eq]) job
+      | `leanExe =>
+        let `exe := facetName
+          | error s!"invalid target '{self}': unknown executable facet '{facetName}'"
+        let job : Job LeanExe := cast (by simp [kind_eq]) job
+        let job ← job.bindM fun exe => fetch (.leanExe exe)
+        return cast (by simp [kind_eq]) job
+      | `externLib =>
+        let job : Job ExternLib := cast (by simp [kind_eq]) job
+        match facetName with
+        | `static =>
+          let job ← job.bindM fun lib => fetch (.staticExternLib lib)
+          return cast (by simp [kind_eq]) job
+        | `shared =>
+          let job ← job.bindM fun lib => fetch (.sharedExternLib lib)
+          return cast (by simp [kind_eq]) job
+        | `dynlib =>
+          let job ← job.bindM fun lib => fetch (.dynlibExternLib lib)
+          return cast (by simp [kind_eq]) job
+        | _ =>
+          error s!"invalid target '{self}': unknown external library facet '{facetName}'"
+      | _ =>
+        error s!"invalid target '{self}': unknown data kind '{dataKind}'"
+
+@[inline] protected def BuildKey.fetch
+  (self : BuildKey) [FamilyOut BuildData self α] : FetchM (Job α)
+:= cast (by simp) self.fetchCore
 
 @[inline] protected def Target.fetch (self : Target α) : FetchM (Job α) := do
  have := self.data_def; self.key.fetch
